\documentclass[aps,12pt]{revtex4}
\usepackage[a4paper]{geometry}
\usepackage{graphicx}
\usepackage{amssymb,amsfonts,amsmath,amsthm}
\usepackage{bm}
\usepackage{pslatex}
\usepackage{chemarr}
\usepackage{mathptmx}
\usepackage{bookman}

  	 
\begin{document}

\section{Preamble}

\begin{itemize}
	\item enzyme definition and role
	\item $k_{obs}$ in function of diffusion time and conversion time
	\item Intermédiaire Réactionnel / Etat de transition
\end{itemize}

\section{Fully Reversible}



\subsection{Equations}

\begin{equation}
	E + S \xrightleftharpoons[k_d]{k_f} ES 
	\xrightleftharpoons[k_r]{k_p} P + E
\end{equation}

\begin{equation}
\left\lbrace
\begin{array}{rcl}
	v_f & =  & k_f [E][S] \\
	v_d & =  & k_d [ES]   \\
	v_p & =  & k_p [ES]   \\
	v_r & =  & k_r [P][E]  \\
\end{array}
\right.
\end{equation}

\begin{equation}
\left\lbrace
\begin{array}{rcl}
  \partial_t [E]  & = & v_d - v_f + v_p - v_r\\
  \partial_t [S]  & = & v_d - v_f = \partial_t [E]\\
  \partial_t [ES] & = & v_f - v_d - v_p + v_r\\ 
  \partial_t [P]  & = & v_p - v_r\\
\end{array}
\right.
\end{equation}

\begin{equation}
	\partial_t 
	\begin{bmatrix}
		[E]  \\
		[S]  \\
		[ES] \\
		[P]  \\
	\end{bmatrix}
	=	
	\partial_t \vec C = 
	\begin{bmatrix}
	-1 &  1 &  1 & -1 \\
	-1 &  1 &  0 &  0 \\
	 1 & -1 & -1 &  1 \\
	 0 &  0 &  1 & -1 \\
	\end{bmatrix}
	\begin{bmatrix}
		v_f\\
		v_d\\
		v_p\\
		v_r\\
	\end{bmatrix}
\end{equation}

rank=2

\subsection{Conservations}
\begin{equation}
	\partial_t ( [E] + [ES] ) = 0 \implies E_0 = [E] + [ES]
\end{equation}

\begin{equation}
	\partial_t ( [S] + [ES] + [P]) = 0 \implies S_0 = [S] + [ES] + [P]
\end{equation}

\subsection{Steady States}

\begin{equation}
\left\lbrace
\begin{array}{rcl}
	k_f [E]_\star[S]\star & = & k_d [ES]_\star\\
	k_p [ES]_\star        & = & k_r [P]_\star[E]_\star \\
\end{array}
\right.
\end{equation}

\begin{equation}
	K_1 = \dfrac{k_d}{k_f} \;\;\;\; K_2 = \dfrac{k_r}{k_p}\\
\end{equation}

\begin{equation}
\left\lbrace
\begin{array}{rcl}
 		~[ES]_\star & = & \dfrac{[E]_\star[S]_\star}{K_1} \\
		\\
		~[E]_\star  & = & \dfrac{E_0K_1}{ [S]_\star + K_1} \\
		\\
		~[P]_\star  & = & \dfrac{[S]_\star}{K_1K_2}\\
		\\
		S_0 & = & \dfrac{E_0 [S]_\star}{[S]_\star+K_1} + \dfrac{[S]_\star}{K_1K_2} + [S]_\star
\end{array}
\right.
\end{equation}

\subsection{Catalytic Irreversible}

\begin{itemize}
	\item $v_r\equiv 0$
	\item no steady state
	\item no equilibrium
	%\item $[S]+[P]\gg[E],[ES]$
\end{itemize}

\begin{equation}
	E + S \xrightleftharpoons[k_d]{k_f} ES 
	\xrightleftharpoons[0]{k_p} P + E
\end{equation}

\begin{equation}
\left\lbrace
\begin{array}{rcl}
  \partial_t [E]  & = & v_d - v_f + v_p \\
  \partial_t [S]  & = & v_d - v_f \\
  \partial_t [ES] & = & v_f - v_d - v_p \\ 
  \partial_t [P]  & = & v_p \\
\end{array}
\right.
\end{equation}

\begin{equation}
\left\lbrace
\begin{array}{rcl}
 E_0 & = & [E] + [ES]\\
 S_0 & = & [S] + [ES] + [P] \\ %\simeq [S]+[P]\\
 \end{array}
 \right.
\end{equation}

\begin{equation}
\left\lbrace
\begin{array}{rcl}
\partial_t [ES] & = & k_f [S] [E] - (k_d+k_p) [ES]\\
                & = & k_f [S] (E_0-[ES]) - (k_d+k_p) [ES]\\
                & = & k_f [S] E_0 - (k_f [S] + (k_d+k_p)) [ES]\\
                \\
\partial_t [S] & = & k_d[ES] - k_f [S][E] \\
               & = & k_d[ES] - k_f [S](E_0 - [ES])\\
               & = & (k_d+k_f[S])[ES] - k_f[S]E_0 \\
\end{array}
\right.
\end{equation}

\begin{itemize}
	\item S is consumed $\implies \partial_t [S] < 0 \implies [S]$ decreasing
	\item $\partial_t [ES]_0 = k_f E_0 S_0 > 0$
	\item $\partial_t [ES]_\infty \simeq - (k_d+k_p) [ES]_\infty$: there exist a moment when it's negative
	\item There is at least one moment when $\partial_t [ES]=0$, existence.
\end{itemize}

\begin{equation}
	K_M = \dfrac{k_d+k_p}{k_f}
\end{equation}

\begin{equation}
	\partial_t [ES] = k_f( [S]E_0 - ([S]+K_M) [ES] )
\end{equation}

\begin{equation}
	[ES] \simeq E_0 \dfrac{[S]}{[S]+K_M}
\end{equation}


\end{document}