\documentclass[aps,12pt]{revtex4}
\usepackage[a4paper]{geometry}
\usepackage{graphicx}
\usepackage{amssymb,amsfonts,amsmath,amsthm}
\usepackage{bm}
\usepackage{pslatex}
\usepackage{chemarr}
\usepackage{mathptmx}
\usepackage{bookman}

  	 
\begin{document}

Let  $\vec{M}(s)$ be an arc of $\mathbb{R}^2$,  $\vec{T}(s) = \partial_s \vec{M}$, $\theta(s) = \widehat{(\vec{i},\vec{T})}$.

\begin{equation}
	\vec{T} = 
	\begin{bmatrix}
	\cos \theta\\
	\sin \theta
	\end{bmatrix}
\end{equation}

\begin{equation}
	\partial_s \vec{T} = \partial_s \theta 
	\begin{bmatrix}
	-\sin\theta\\
	\cos \theta
	\end{bmatrix}
 = \gamma \vec{N}
\end{equation}

The distance of $\vec{M}_k$ to $\mathcal{C}$ is: 
\begin{equation}
	d^2_k(s) = \left[ \vec{M}_k - \vec{M}_0 - s \vec{T}\right]^2 = \left[ \vec{\delta}_k - s \vec{T}\right]^2
	=  \vec{\delta}_k^2 - 2 s  \vec{\delta}_k \cdot \vec{T} + s^2
\end{equation}
It is minimal when:
\begin{equation}
	s^\star = \vec{\delta}_k \cdot \vec{T}
\end{equation}
so that:
\begin{equation}
	d^2_k = \vec{\delta}_k^2 - \left(\vec{\delta}_k \cdot \vec{T} \right)^2  
\end{equation}

\begin{equation}
 	d^2_k =  (x_k-x_0)^2 + (y_k -y_0)^2 - \left[ (x_k-x_0)\cos\theta_0 + (y_k-y_0)\sin\theta_0\right]^2
\end{equation}

\begin{equation}
\left\lbrace
\begin{array}{rcl}
\partial_{x_0} \frac{1}{2} d^2_k & = & -(x_k-x_0) + \cos\theta_0 \left[ (x_k-x_0)\cos\theta_0 + (y_k-y_0)\sin\theta_0\right]\\
\\
\partial_{x_0} \frac{1}{2} d^2_k & = & -(y_k-y_0) + \sin\theta_0 \left[ (x_k-x_0)\cos\theta_0 + (y_k-y_0)\sin\theta_0\right]\\
\\
\partial_{\theta_0} \frac{1}{2} d^2_k & = & -\left[ (x_k-x_0)\cos\theta_0 + (y_k-y_0)\sin\theta_0\right]\left[ -(x_k-x_0)\sin\theta_0 + (y_k-y_0)\cos\theta_0\right]\\
\end{array}
\right.
\end{equation}

\begin{equation}
\left\lbrace
\begin{array}{rcl}
\sum_k\partial_{x_0} \frac{1}{2} d^2_k & = & 0\\
\sum_k\partial_{y_0} \frac{1}{2} d^2_k & = & 0\\
\end{array}
\right.
\iff
\left\lbrace
\begin{array}{rcl}
x_0 & = & \bar{x} \\
y_0 & = & \bar{y} \\
\end{array}
\right.
\end{equation}

\begin{equation}
\partial_{\theta_0} \frac{1}{2} d^2_k = \left[ (x_k-x_0)^2-(y_k-y_0)^2 \right] \cos\theta_0\sin\theta_0 - (x_k-x_0) (y_k-y_0) \left[ \cos^2\theta_0 - \sin^2\theta_0\right]
\end{equation}

\begin{equation}
\partial_{\theta_0} \frac{1}{2} d^2_k = \left[ (x_k-x_0)^2 - (y_k-y_0)^2\right] \frac{1}{2} \sin 2\theta_0 - (x_k-x_0) (y_k-y_0) \cos 2\theta_0
\end{equation}

\begin{equation}
0 = \sum_k\partial_{\theta_0} \frac{1}{2} d^2_k \implies 0 = \left[ \sigma_x^2 - \sigma_y^2 \right] \frac{1}{2} \sin 2\theta_0 - \sigma_{xy} \cos 2\theta_0
\end{equation}

\end{document}