\documentclass[aps,12pt]{revtex4}
\usepackage[a4paper]{geometry}
\usepackage{graphicx}
\usepackage{amssymb,amsfonts,amsmath,amsthm}
\usepackage{bm}
\usepackage{pslatex}
\usepackage{chemarr}
\usepackage{mathptmx}
\usepackage{bookman}

  	 
\begin{document}


\section{Correcting Conservation}

Let $\vec{\alpha}\in\mathbb{N}_+^M$ be a conservation vector, meaning that for any $\vec{C}_0$:
\begin{equation}
d\,\left(\langle \vec{\alpha} \vert \vec{C}_0 \rangle\right) = 0.
\end{equation}
In particular:
\begin{equation}
	\langle \vec{\alpha} \vert \vec{C}_0 \rangle \geq 0.
\end{equation}

Let us assume that we start from:
\begin{equation}
	\langle \vec{\alpha} \vert \vec{C}_0 \rangle < 0.
\end{equation}
We compute the smallest numerical correction $\delta\vec{C}$ such that:
\begin{equation}
	\langle \vec{\alpha} \vert \vec{C}_0 + \delta\vec{C} \rangle = 0.
\end{equation}
We find:
\begin{equation}
	\delta\vec{C} =
	 -\dfrac{\langle \vec{\alpha} \vert \vec{C}_0 \rangle}{\vec{\alpha}^2}
	  \vec{\alpha}.
\end{equation}

\begin{equation}
	\delta\vec{C}^2 = \dfrac{\langle \vec{\alpha} \vert \vec{C}_0 \rangle^2}{\vec{\alpha}^2}
\end{equation}

\begin{equation}
	\vec{C}_0' = \vec{C_0} - \delta\vec{C} = \dfrac{1}{\vec{\alpha}^2}
	\left[ \vec{\alpha}^2 \bm{I} - \vert \vec{\alpha} \rangle \langle \vec{\alpha} \vert \right] \vec{C}_0
\end{equation}

\end{document}

In that case we obtain:
\begin{equation}
	\vec{C}_0' = \vec{C}_0 - \delta\vec{C},\; \vec{C}_0' \in \vec{\alpha}^\perp
\end{equation}	
	
Let assume that we know $\lbrace \vec{\beta}_i \rbrace$  vectors of $\mathbb{Z}^M$ as an orthogonal basis of $\vec{\alpha}^\perp$:
\begin{equation}
	\forall i,\; \langle \vec{\beta}_i \vert \vec{\alpha} \rangle = 0, \;\; \forall j\not=i,\;\langle \vec{\beta}_i \vert \vec{\beta}_j \rangle = 0
\end{equation}
then
\begin{equation}
	\vec{C}_0' = \sum_i b_i \vec{\beta}_j \implies b_i = \dfrac{\langle \vec{\beta}_i \vert \vec{C}_0 \rangle}{\vec{\beta}_i^2}
\end{equation}
and
\begin{equation}
	\vec{C}_0' = \sum_i \dfrac{\langle \vec{\beta}_i \vert \vec{C}_0 \rangle}{\vec{\beta}_i^2} \vec{\beta}_i = \left( \right) \vec{C}_0
\end{equation}
	
%\begin{equation}
%	\vert\delta\vec{C}\vert = \dfrac{-\langle \vec{\alpha} \vert \vec{C}_0 \rangle}{\vert \vec{\alpha} \vert}
%\end{equation}	

\end{document}