\documentclass[aps,12pt]{revtex4}
\usepackage[a4paper]{geometry}
\usepackage{graphicx}
\usepackage{amssymb,amsfonts,amsmath,amsthm}
\usepackage{bm}
\usepackage{pslatex}
\usepackage{chemarr}
\usepackage{mathptmx}
\usepackage{bookman}
\usepackage{esint}
\usepackage{xfrac}  	 
	 
\newcommand{\half}{\frac{1}{2}}
	 
\begin{document}

\section{Conservations}

\subsection{One Conservation}

Let us assume that the conservation $\vec \alpha \in \mathbb{N}_\ast^M$ is not fulfilled:

\begin{equation}
	\langle \vec \alpha \vert \vec C \rangle = - X_s, \; X_s > 0
\end{equation}

We also assume that this conservation concerned a set of $N$ equilibrium(a) (with possible combination(s))
with a topology:
\begin{equation}
	\bm \nu \in \mathcal{M}_{N,M}  \end{equation}
and:

\begin{equation}
	 \bm \nu ^T \vec \alpha = \vec 0
\end{equation}

The conservation correction is:
\begin{equation}
	\delta \vec C =  \dfrac{X_s}{\vec\alpha^2} \vec \alpha  
\end{equation}
and we obtain:
\begin{equation}
	\vec C ' = \vec C + \delta \vec{C}
\end{equation}
 
\subsection{Multiple Conservations}

\begin{equation}
	\forall i \in [1:n], \; \langle \vec \alpha_i \vert \vec C \rangle = -X_i, \; X_i > 0
\end{equation}

We look for the minimal $\delta \vec  C$ such that:

\begin{equation}
	\forall i \in [1:n], \; \langle \vec \alpha_i \vert \vec C + \delta \vec C \rangle = 0 = \langle \vec \alpha_i \vert \delta \vec C \rangle - X_i
\end{equation}

\begin{equation}
	L(\delta \vec C) = \dfrac{1}{2} \delta \vec C ^2 - \sum_i\lambda_i \left( \langle \vec \alpha_i \vert \delta \vec C \rangle - X_i\right)
\end{equation}

\begin{equation}
	\vec 0 = \delta \vec C - \sum_i \lambda_i \vec\alpha_i
\end{equation}

\begin{equation}
	\bm{A} = 
	\begin{bmatrix}
	\vdots\\
	\langle \vec \alpha_i \vert \\
	\vdots
	\end{bmatrix}
\end{equation}

\begin{equation}
	\delta \vec C = \bm{A}^T \vec \lambda
\end{equation}

\begin{equation}
	\bm{A} \delta \vec C = \vec X = \left(\bm{A} \bm{A}^T\right) \lambda
\end{equation}

\begin{equation}
	\delta \vec{C} = \bm{A}^T \left(\bm{A} \bm{A}^T\right)^{-1} \vec{X} = \bm{A}^T \left(\bm{A} \bm{A}^T\right)^{-1} \bm{A} \vec{C}
\end{equation}

\end{document}