\documentclass[aps,12pt]{revtex4}
\usepackage[a4paper]{geometry}
\usepackage{graphicx}
\usepackage{amssymb,amsfonts,amsmath,amsthm}
\usepackage{bm}
\usepackage{pslatex}
\usepackage{chemarr}
\usepackage{mathptmx}
\usepackage{bookman}

  	 
\begin{document}

\section{Three Points}

Let $\vec{A}, \vec{B}, \vec{C}$ be three points on an arc.
If $a,b,c$ are the length of the segments, then the semi-perimeter $s$ is:
\begin{equation}
s = \dfrac{a+b+c}{2},
\end{equation}
and the diameter of the circumcircle is:
\begin{equation}
	d = \dfrac{abc}{2\sqrt{s(s-a)(s-b)(s-c)}} = \dfrac{2abc}{\sqrt{(a+b+c)(a+b-c)(a-b+c)(-a+b+c)}}.
\end{equation}
The curvature is:
\begin{equation}
	\kappa = \dfrac{\sqrt{(a+b+c)(a+b-c)(a-b+c)(-a+b+c)}}{abc}
\end{equation}

\section{Circular Spline}

\subsection{Definition}

On $[i;i+1]$:
\begin{equation}
	\vec{P}(t) = (1-t) \vec{P}_i + t \vec{P}_{i+1} + E(t) \vec{P}'''_i + F(t) \vec{P}'''_{i+1}
\end{equation}
such that
\begin{equation}
	\vec{P}'''(t) = (1-t) \vec{P}'''_i + t \vec{P}'''_{i+1}
\end{equation}

\begin{equation}
	Q(t,q) = \dfrac{t^4 - (1+q) t ^2 + q  t}{24} = \dfrac{t}{24}\left[ t^3 - (1+q) t + q\right]
\end{equation}

Functions:
\begin{equation}
\left\lbrace
\begin{array}{rcl}
	F(t) & = &Q(t,\beta)\\
	E(t) & = &-Q(1-t,\alpha)\\
\end{array}
\right.
\end{equation}

First Derivatives:
\begin{equation}
\left\lbrace
\begin{array}{rcccl}
	F'(t) & = &Q'(t,\beta) & = & \dfrac{4t^3 - 2(1+\beta) t  + \beta  }{24}\\
	\\
	E'(t) & = &\left[-Q(1-t,\alpha)\right]' & = & Q'(1-t,\alpha)\\
\end{array}
\right.
\end{equation}

Second Derivatives:
\begin{equation}
\left\lbrace
\begin{array}{rcccl}
	F''(t) & = &Q''(t,\beta) & = & \dfrac{6t^2 - (1+\beta) }{12}\\
	\\
	E''(t) & = &\left[-Q(1-t,\alpha)\right]'' & = & -Q''(1-t,\alpha)\\
\end{array}
\right.
\end{equation}

\subsection{Continuity of first derivatives}

\begin{equation}
	\vec{P}'_i 
	 = \vec{P}_{i+1} - \vec{P}_i + E'_i(0) \vec{P}'''_i + F'_i(0) \vec{P}'''_{i+1} 
	 = \vec{P}_i - \vec{P}_{i-1} + E'_{i-1}(1) \vec{P}'''_{i-1} + F'_{i-1}(1) \vec{P}'''_i
\end{equation}

\begin{equation}
	\vec{P}_{i-1} - 2 \vec{P}_i + \vec{P}_{i+1} 
	=  \left[E'_{i-1}(1)\right] \vec{P}'''_{i-1} + \left[F'_{i-1}(1)- E'_i(0)\right] \vec{P}'''_i + \left[- F'_i(0)\right] \vec{P}'''_{i+1} 
\end{equation}


\end{document}