\documentclass[aps,12pt]{revtex4}
\usepackage[a4paper]{geometry}
\usepackage{graphicx}
\usepackage{amssymb,amsfonts,amsmath,amsthm}
\usepackage{bm}
\usepackage{pslatex}
\usepackage{chemarr}
\usepackage{mathptmx}
\usepackage{bookman}

  	 
\begin{document}

\section{Notations}
Let us assume that we have local minimum defined by a triplet of coordinates such that:
\begin{equation}
	x_a \leq x_b \leq x_c \text{ and } f_b \leq f_a \text{ and } f_b \leq f_c
\end{equation}

We change the coordinate to $u_a=0$, $u_c=1$ and
\begin{equation}
	\beta = \left\lbrace
	\begin{array}{cc}
	0 & \iff  x_b\leq x_a\\
	1 & \iff  x_c\leq x_b\\
	\dfrac{x_b-x_a}{x_c-x_a} & \iff x_a < x_b < x_c\\
	\end{array}
	\right.
\end{equation}

\section{Parabola}
\subsection{Notations}
We define the reduced polynomial
\begin{equation}
	Q(u) =  \mu_a (1-u) + \mu_c u - \gamma u(1-u)
\end{equation}	 
 
\begin{equation}
\begin{array}{rcl}
	Q(0) & = & \mu_a = f_a - f_b \geq 0\\
	Q(1) & = & \mu_c = f_c - f_b \geq 0\\
	Q(\beta) & = & 0 = (1-\beta)\mu_a + \beta \mu_c - \gamma \beta(1-\beta)\\
\end{array}
\end{equation}	

\begin{equation}
	\gamma = \dfrac{(1-\beta)\mu_a + \beta \mu_c}{\beta(1-\beta)}  \geq 0 
\end{equation}

\subsection{Quadratic Minimum}
\begin{equation}
\boxed{
	u_\star = \dfrac{1}{2} + \dfrac{\mu_a-\mu_c}{2\gamma} = \dfrac{1}{2} + \dfrac{\beta(1-\beta)}{2} 
	\dfrac{\mu_a-\mu_c}{(1-\beta)\mu_a + \beta \mu_c}
	}
\end{equation}

\subsection{Reduction}
We look for the reduction position $u_\bullet$ for which $\mu_{a,new}=\mu_{c,new}$.

\begin{equation}
\left\lbrace
\begin{array}{rcll}
	\mu_a & = & \mu_a (1-u) + \mu_c u - \gamma u(1-u) , & \mu_c \geq \mu_a\\
	\mu_c & = & \mu_a (1-u) + \mu_c u - \gamma u(1-u) , & \mu_c \leq \mu_a\\
\end{array}
\right.
\end{equation}	 

\begin{equation}
\left\lbrace
\begin{array}{rcll}
	0     & = &    (\mu_c-\mu_a)  - \gamma (1-u), & \mu_c \geq \mu_a\\
	0 & = & (\mu_a -\mu_c)   - \gamma u         , & \mu_c \leq \mu_a\\
\end{array}
\right.
\end{equation}	 

\begin{equation}
\left\lbrace
\begin{array}{rcll}
	u_\bullet    & = &   1+ (\mu_a-\mu_c) / \gamma, & \mu_c \geq \mu_a\\
	u_\bullet   & = & (\mu_a -\mu_c)/\gamma,       & \mu_c \leq \mu_a\\
\end{array}
\right.
\end{equation}	

\subsection{Summary}
\begin{equation}
\delta = (\mu_a -\mu_c)/\gamma = \beta(1-\beta)
	\dfrac{\mu_a-\mu_c}{(1-\beta)\mu_a + \beta \mu_c}
\end{equation}

\begin{itemize}
\item Special Cases:

\begin{equation}
\begin{array}{lcl}
\beta \leq 0           & \implies & u_\star = \dfrac{1}{2} \text{, no $u_\bullet$}\\
\\
\beta \geq 1           & \implies & u_\star = \dfrac{1}{2} \text{, no $u_\bullet$}\\
\end{array}
\end{equation}

\item Generic Cases $0<\beta<1$:
\begin{equation}
\begin{array}{lcll}
\mu_a = 0, \;\mu_c = 0 & \implies & u_\star = \dfrac{1}{2}, & \text{no $u_\bullet$}\\
\\
\mu_a > 0, \;\mu_c = 0 & \implies & u_\star = \dfrac{1}{2} + \dfrac{\beta}{2}, &\; u_\bullet=\beta \\
\\
\mu_a = 0, \;\mu_c > 0 & \implies & u_\star = \dfrac{\beta}{2}, & u\bullet = 1 - \beta \\
\\
\mu_a \simeq \mu_c & \implies & u_\star = \dfrac{1}{2}, & \text{no $u_\bullet$} \\
\end{array}
\end{equation}

\end{itemize}



 



\end{document}