\documentclass[aps,12pt]{revtex4}
\usepackage[a4paper]{geometry}
\usepackage{graphicx}
\usepackage{amssymb,amsfonts,amsmath,amsthm}
\usepackage{bm}
\usepackage{pslatex}
\usepackage{chemarr}
\usepackage{mathptmx}
\usepackage{bookman}
\usepackage{array}
  	 
\begin{document}

Let $\vec{z}_1,\ldots,\vec{z}_n$ be points taken at "times" $t_i$ and
we want to fit them at $t_0$ with a low degree polynomial of degree $d$,
with $m=d+1$ coefficients:
\begin{equation}
P(t) = \vec{z}_0 + \sum_{k=0}^{d} \left(t-t_0\right)^k \vec{a}_k
\end{equation}


\begin{equation}
	D^2 = \dfrac{1}{2} \sum_{i=1}^n
	\left[ 
	\left(\vec{z}_i - \vec{z}_0\right) -
	\left(\sum_{k=0}^{d} \left(t_i-t_0\right)^k \vec{a}_k \right)
	 \right]^2
\end{equation}	

\begin{equation}
	\forall\; 0 \leq l \leq d,\;
	\partial_{\vec{a}_l} D^2 =
	-\sum_{i=1}^n  \left(t_i-t_0\right)^l \left[ 
	\left(\vec{z}_i - \vec{z}_0\right) -
	\left(\sum_{k=0}^{d} \left(t_i-t_0\right)^k \vec{a}_k \right)
	 \right]
\end{equation}

\begin{equation}
	\forall\; 0 \leq l \leq d,\;
	\sum_{k=0}^{d} \left[ \sum_{i=1}^n \left(t_i-t_0\right)^{(k+l)} \right] \vec{a}_k = 
	\sum_{i=1}^n \left(t_i-t_0\right)^l  
	\left(\vec{z}_i - \vec{z}_0\right)
\end{equation}

\begin{equation}
\left[ \sum_{k=1}^n (t_k-t_0)^{i+j-2}\right] \vec{A} = 
\begin{bmatrix}
\sum_{k=1}^n\left(\vec{z}_k - \vec{z}_0\right) \\
\sum_{k=1}^n\left(t_k-t_0\right)\left(\vec{z}_k - \vec{z}_0\right)\\
\vdots\\
\sum_{k=1}^n\left(t_k-t_0\right)^{j-1}\left(\vec{z}_k - \vec{z}_0\right)\\
\vdots\\
\sum_{k=1}^n\left(t_k-t_0\right)^{d-1}\left(\vec{z}_k - \vec{z}_0\right)\\
\end{bmatrix}
\end{equation}

We choose:
\begin{equation}
	\vec{z}_0 = \frac{1}{n} \sum_{k=1}^n \vec{z}_k
\end{equation}
so that:
\begin{equation}
	\sum_{k=1}^n\left(\vec{z}_k - \vec{z}_0\right) = \vec{0}
\end{equation}

\end{document}

Let $\vec{z}_1,\ldots,\vec{z}_n$ be points taken at "times" $t_i=i$ and
we want to fit them at $t_j,\vec{z}_j$ with:
\begin{equation}
	\vec{z} = \vec{P}(t-t_j) + \vec{z}_j, \; P(u) = \sum_{k=0}^{p<n} u^k \vec{a}_k
\end{equation}
We want to minimize:
\begin{equation}
	D^2 = \dfrac{1}{2} \sum_{i=1}^n \left\vert
	\left(\vec{z}_i - \vec{z}_j\right) - \vec{P}(t_i-t_j)
	\right\vert^2 = \dfrac{1}{2} \sum_{i=1}^n \left\vert \left(\vec{z}_i - \vec{z}_j\right)  - \sum_{k=0}^{p<n} (t_i-t_j)^k \vec{a}_k
	\right\vert^2
\end{equation}

\begin{equation}
	\partial_{\vec{a}_l} D^2 = \sum_{i=1}^n (t_i-t_j)^l \left( \left(\vec{z}_i - \vec{z}_j\right)  
	- \sum_{k=0}^{p<n} (t_i-t_j)^k \vec{a}_k \right)
\end{equation}

\begin{equation}
\forall 0 \leq l \leq p, \;\; \sum_{i=1}^n  \sum_{k=0}^{p<n} (t_i-t_j)^{k+l} \, \vec{a}_k 
= \sum_{i=1}^n (t_i-t_j)^l \left(\vec{z}_i - \vec{z}_j\right) 
\end{equation}

\begin{equation}
	\sum_{k=0}^{p} \left[\sum_{i=1}^n (t_i-t_j)^{k+l} \right] \vec{a}_k = \sum_{i=1}^n (t_i-t_j)^l \left(\vec{z}_i - \vec{z}_j\right) 
\end{equation}

\begin{equation}
	\sum_{k=0}^{p} \bm{\mu}_{l,k} \vec{a}_k = \vec{w}_l \otimes \vec{Z}
\end{equation}
	

\begin{equation}
	\bm{\mu} \vec{A} = \bm{W} \vec{Z},\;\;\bm{\mu} \in \mathcal{M}_{p,p}.\;\;\bm{W} \in \mathcal{M}_{p,n}
\end{equation}

\begin{equation}
	\vec{A} = \left(\bm{\mu}^{-1}\bm{W}\right) \vec{Z}
\end{equation}

\end{document}