\documentclass[aps,12pt]{revtex4}
\usepackage[a4paper]{geometry}
\usepackage{graphicx}
\usepackage{amssymb,amsfonts,amsmath,amsthm}
\usepackage{bm}
\usepackage{pslatex}
\usepackage{chemarr}
\usepackage{mathptmx}
\usepackage{bookman}

  	 
\begin{document}

\section{Three Points}

Let $\vec{A}, \vec{B}, \vec{C}$ be three points on an arc.
If $a,b,c$ are the length of the segments, then the semi-perimeter $s$ is:
\begin{equation}
s = \dfrac{a+b+c}{2},
\end{equation}
and the diameter of the circumcircle is:
\begin{equation}
	d = \dfrac{abc}{2\sqrt{s(s-a)(s-b)(s-c)}} = \dfrac{2abc}{\sqrt{(a+b+c)(a+b-c)(a-b+c)(-a+b+c)}}.
\end{equation}
The curvature is:
\begin{equation}
	\kappa = \dfrac{\sqrt{(a+b+c)(a+b-c)(a-b+c)(-a+b+c)}}{abc}
\end{equation}

\section{Cubic Splines}

\subsection{Linear Interpolation}
Let $\vec{y}_1,\ldots,\vec{y}_{N}$ be $N$ points at $t_1<\ldots<t_N$.
The linear interpolation gives:
\begin{equation}
\left\lbrace
\begin{array}{rcl}
	\vec{y} & = & A \, \vec{y}_i + B \, \vec{y}_{i+1} \\
	\\
	A & = & \dfrac{t_{i+1}-t}{t_{i+1}-t_i}, \; A(t_i) = 1,\;A(t_{i+1})=0\\
	\\
	B & = & \dfrac{t-t_i}{t_{i+1}-t_i}, \; B(t_i) = 0,\;B(t_{i+1})=1\\
	\end{array}
\right.
\end{equation}


\subsection{Cubic Interpolation}

\subsubsection{Generic Case}

\begin{equation}
\left\lbrace
\begin{array}{rcl}
	\vec{y}   & = & A \, \vec{y}_i + B \, \vec{y}_{i+1} + C \, \vec{y}_i'' + D \, \vec{y}_{i+1}''\\
	\\
	C & = & \frac{1}{6} \left(A^3 - A\right) (t_{i+1}-t_i)^2\\
	\\
	D & = & \frac{1}{6} \left(B^3 - B\right) (t_{i+1}-t_i)^2\\
\end{array}
\right.
\end{equation}

\begin{equation}
	\vec{y}' = \dfrac{1}{t_{i+1}-t_i} \left(\vec{y}_{i+1}-\vec{y}_i\right) 
	- \dfrac{3A^2-1}{6} (t_{i+1}-t_i) \vec{y}_i''
	+ \dfrac{3B^2-1}{6} (t_{i+1}-t_i) \vec{y}_{i+1}''
\end{equation}	


\begin{equation}
	\vec{y}'' = A \vec{y}_i'' + B \vec{y}_{i+1}''
\end{equation}

The first derivative continuity yields $\forall 2\leq i \leq N-1$:
\begin{equation}
 	\dfrac{t_{i}-t_{i-1}}{6} \vec{y}_{i-1}'' + 
	\dfrac{t_{i+1}-t_{i-1}}{3} \vec{y}_i''
	+\dfrac{t_{i+1}-t_{i}}{6} \vec{y}_{i+1}''  = 
	\dfrac{1}{t_{i+1}-t_i} \left( \vec{y}_{i+1} - \vec{y}_{i} \right) -
	\dfrac{1}{t_{i}-t_{i-1}} \left( \vec{y}_i - \vec{y}_{i-1} \right) 
\end{equation}


\subsubsection{Linear Case}
The boundary conditions may be natural or with fixed first derivatives.
\begin{itemize}
\item At $\vec{y}_1$:
\begin{equation}
	\vec{y}_1'' = \vec{0} 
\end{equation}
or
\begin{equation}
\vec{y}'_1 = \dfrac{1}{t_{2}-t_1} \left(\vec{y}_{2}-\vec{y}_1\right) 
	- \dfrac{3A(t_1)^2-1}{6} (t_{2}-t_1) \vec{y}_1''
	+ \dfrac{3B(t_1)^2-1}{6} (t_{2}-t_1) \vec{y}_{2}''
\end{equation}
and with $A(t_1)=1,\,B(t_1)=0$:
\begin{equation}
\vec{y}'_1  = \dfrac{1}{t_{2}-t_1} \left(\vec{y}_{2}-\vec{y}_1\right) 
	+ \dfrac{1}{3} (t_{2}-t_1) \vec{y}_1''
	- \dfrac{1}{6} (t_{2}-t_1) \vec{y}_{2}''
\end{equation}
 
\item At $\vec{y}_N$:
\begin{equation}
	\vec{y}_N'' = \vec{0} 
\end{equation}
or
\begin{equation}
\vec{y}_N' = \dfrac{1}{t_{N}-t_{N-1}} \left(\vec{y}_{N}-\vec{y}_{N-1}\right) 
	- \dfrac{3A^2-1}{6} (t_{N}-t_{N-1}) \vec{y}_{N-1}''
	+ \dfrac{3B^2-1}{6} (t_{N}-t_{N-1}) \vec{y}_{N}''
\end{equation}
and with $A(t_N)=0,\,B(t_N)=1$:
\begin{equation}
	\vec{y}_N' =  \dfrac{1}{t_{N}-t_{N-1}} \left(\vec{y}_{N}-\vec{y}_{N-1}\right) 
	+ \dfrac{1}{6} (t_{N}-t_{N-1}) \vec{y}_{N-1}''
	+ \dfrac{1}{3} (t_{N}-t_{N-1}) \vec{y}_{N}''
\end{equation}
\end{itemize}

\subsubsection{Cyclic Case}
\begin{itemize}
\item We need to define $t_{0}$ to write:
\begin{equation}
 	\dfrac{t_{1}-t_{0}}{6} \vec{y}_{N}'' + 
	\dfrac{t_{2}-t_{0}}{3} \vec{y}_1''
	+\dfrac{t_{2}-t_{1}}{6} \vec{y}_{2}''  = 
	\dfrac{1}{t_{2}-t_1}   \left( \vec{y}_{2} - \vec{y}_{1} \right) -
	\dfrac{1}{t_{1}-t_{0}}  \left( \vec{y}_1 - \vec{y}_{0} \right) 
\end{equation}

\item We need to define $t_{N+1}$ to write:
\begin{equation}
 	\dfrac{t_{N}-t_{N-1}}{6} \vec{y}_{N-1}'' + 
	\dfrac{t_{N+1}-t_{N-1}}{3} \vec{y}_i''
	+\dfrac{t_{N+1}-t_{N}}{6} \vec{y}_{1}''  = 
	\dfrac{1}{t_{N+1}-t_N}   \left( \vec{y}_{1} - \vec{y}_{N} \right) -
	\dfrac{1}{t_{N}-t_{N-1}} \left( \vec{y}_N - \vec{y}_{N-1} \right) 
\end{equation}

\end{itemize}

\end{document}